platform/tests/Yield.v
@@ -7,7 +7,7 @@ Import M.
 Module T := Thread0.Make(M).
 Import T.
 
-Definition handlerS := SPEC reserving 26
+Definition handlerS := SPEC reserving 39
   PREmain[_] sched * mallocHeap 0.
 
 Definition mainS := SPEC reserving 49
@@ -19,12 +19,12 @@ Definition m := bimport [[ "scheduler"!"init" @ [initS], "scheduler"!"exit" @ [e
     bfunctionNoRet "handler"("x", "y") [handlerS]
       Yield
       [PREmain[_] sched * mallocHeap 0];;
-      Exit 27
+      Exit 40
     end with bfunctionNoRet "main"("x", "y") [mainS]
       Init
       [PREmain[_] sched * mallocHeap 0];;
 
-      Spawn("test"!"handler", 27)
+      Spawn("test"!"handler", 40)
       [PREmain[_] sched * mallocHeap 0];;
 
       Go 50
